lean4/Automaton/NFA/Basic.lean
@@ -12,7 +12,7 @@ import Mathlib.Data.FinEnum
 namespace NFA
 
 structure NFA (σs : Finset σ) (qs : Finset q) where
-  init : qs        -- initial state
+  s : qs        -- initial state
   fs : Finset qs   -- accepting states
   δ : qs → σs → Finset qs -- transition function
 
@@ -33,7 +33,7 @@ def δ_star' (q : Finset qs) : (w : word σs) → Finset qs
   | e :: es => δ_star' (δ_step t q e) es
 
 @[simp]
-def δ_star : (w : word σs) → Finset qs := δ_star' t {t.init}
+def δ_star : (w : word σs) → Finset qs := δ_star' t {t.s}
 
 -- Whether a word is in the language that the NFA accepts
 @[simp]
@@ -41,8 +41,8 @@ def nfa_accepts (w : word σs) : Prop := by
   have inter : Finset qs := (δ_star t w) ∩ t.fs
   exact inter.Nonempty
 
--- nfa accepts nil iff init is final
-theorem nfa_accepts_nil_iff_final : nfa_accepts t [] ↔ t.init ∈ t.fs := by
+-- nfa accepts nil iff s is final
+theorem nfa_accepts_nil_iff_final : nfa_accepts t [] ↔ t.s ∈ t.fs := by
   apply Iff.intro
   · intro ne
     simp only [nfa_accepts, δ_star ] at ne
@@ -51,7 +51,7 @@ theorem nfa_accepts_nil_iff_final : nfa_accepts t [] ↔ t.init ∈ t.fs := by
   · intro e
     dsimp [nfa_accepts,δ_star]
     rw [Finset.singleton_inter_of_mem e]
-    exact (Finset.singleton_nonempty t.init)
+    exact (Finset.singleton_nonempty t.s)
 
 instance decidableLang (w : word σs) : Decidable (nfa_accepts t w) := by
   dsimp [nfa_accepts]
